HoareLogic/Sound_Frame.v
@@ -37,10 +37,9 @@ Context {L: Language}
         {minL: MinimumLanguage L}
         {pL: PropositionalLanguage L}
         {sepconL: SepconLanguage L}
-        {wandL: WandLanguage L}
         {SM: Semantics L MD}
         {kiSM: KripkeIntuitionisticSemantics L MD tt SM}
-        {fsSM: FlatSemantics.SeparatingSemantics L MD tt SM}.
+        {fsepconSM: FlatSemantics.SepconSemantics L MD tt SM}.
 
 Lemma hoare_frame_partial_sound: forall c P Q F,
   triple_partial_valid P c Q ->
