SeparationLogic/DeepEmbedded/ParametricCompleteness.v
@@ -66,7 +66,7 @@ Existing Instances ParametricSeparationLogic.GP ParametricSeparationLogic.GD Par
 
 Existing Instances Axiomatization2SequentCalculus_SC Axiomatization2SequentCalculus_bSC Axiomatization2SequentCalculus_fwSC Axiomatization2SequentCalculus_minSC Axiomatization2SequentCalculus_ipSC Axiomatization2SequentCalculus_cpSC.
 
-Existing Instances FlatSemantics.MD FlatSemantics.kMD FlatSemantics.R FlatSemantics.J FlatSemantics.SM FlatSemantics.kminSM FlatSemantics.kpSM FlatSemantics.fsSM FlatSemantics.feSM.
+Existing Instances FlatSemantics.MD FlatSemantics.kMD FlatSemantics.R FlatSemantics.J FlatSemantics.SM FlatSemantics.kminSM FlatSemantics.kpSM FlatSemantics.fsepconSM FlatSemantics.fwandSM FlatSemantics.fempSM.
 
 Definition cP : context -> Prop := Intersection _ (Intersection _ derivable_closed orp_witnessed) consistent.
 
